WIP

AwsCryptographicMaterialProviders/dafny/AwsCryptographyKeyStoreAdmin/src/CreateKeys.dfy
@@ -11,6 +11,7 @@ include "../../AwsCryptographicMaterialProviders/src/AwsArnParsing.dfy"
 include "../../AwsCryptographyKeyStore/src/KmsArn.dfy"
 include "SystemKey/ContentHandler.dfy"
 
+// TODO-HV-2-M1: WIP
 module {:options "/functionSyntax:4" } CreateKeysHV2 {
   // TODO-HV-2-M1-FF: Group imports according to libraries
   import opened StandardLibrary
@@ -36,639 +37,639 @@ module {:options "/functionSyntax:4" } CreateKeysHV2 {
   import CryptoTypes = AwsCryptographyPrimitivesTypes
   import ContentHandler = SystemKey.ContentHandler
 
-  // //= aws-encryption-sdk-specification/framework/branch-key-store.md#branch-key-and-beacon-key-creation
-  // //= type=implication
-  // //# To create a branch key, this operation MUST take the following:
-  // //#
-  // //# - `branchKeyId`: The identifier
-  // //# - `encryptionContext`: Additional encryption context to bind to the created keys
-  // method CreateBranchAndBeaconKeys(
-  //   branchKeyIdentifier: string,
-  //   customEncryptionContext: map<string, string>,
-  //   timestamp: string,
-  //   branchKeyVersion: string,
-  //   logicalKeyStoreName: string,
-  //   kmsConfiguration: Types.KMSConfiguration,
-  //   grantTokens: KMS.GrantTokenList,
-  //   kmsClient: KMS.IKMSClient,
-  //   storage: Types.IKeyStorageInterface
-  // )
-  //   returns (output: Result<Types.CreateKeyOutput, Types.Error>)
-  //   requires 0 < |branchKeyIdentifier|
-  //   requires 0 < |branchKeyVersion|
-  //   requires forall k <- customEncryptionContext :: DDB.IsValid_AttributeName(Structure.ENCRYPTION_CONTEXT_PREFIX + k)
-  //   requires storage.Modifies !! kmsClient.Modifies
-  //   requires KMSKeystoreOperations.HasKeyId(kmsConfiguration) && KmsArn.ValidKmsArn?(KMSKeystoreOperations.GetKeyId(kmsConfiguration))
-
-  //   requires kmsClient.ValidState() && storage.ValidState()
-  //   modifies storage.Modifies, kmsClient.Modifies
-  //   ensures storage.ValidState() && kmsClient.ValidState()
-
-  //   // TODO-HV-2-M1: Update Create Key
-  //   //= aws-encryption-sdk-specification/framework/branch-key-store.md#createkey
-  //   //= type=implication
-  //   //# This operation MUST create a [branch key](structures.md#branch-key) and a [beacon key](structures.md#beacon-key) according to
-  //   //# the [Branch Key and Beacon Key Creation](#branch-key-and-beacon-key-creation) section.
-  //   ensures output.Success?
-  //           ==>
-
-  //             //= aws-encryption-sdk-specification/framework/branch-key-store.md#branch-key-and-beacon-key-creation
-  //             //= type=implication
-  //             //# The call to AWS KMS GenerateDataKeyWithoutPlaintext MUST use the configured AWS KMS client to make the call.
-  //             // The second call is for the beacon key, the first call is the decrypt only. See Seq.Last(Seq.DropLast(
-  //             && |kmsClient.History.Encrypt| == |old(kmsClient.History.Encrypt)| + 3
-  //             && old(kmsClient.History.Encrypt) < kmsClient.History.Encrypt
-
-  //             // TODO-HV-2-M1-FF: Refactor EncryptionContext usage into BranchKeyContext
-  //             && var decryptOnlyEncryptionContext := Structure.DecryptOnlyBranchKeyEncryptionContext(
-  //                                                      branchKeyIdentifier,
-  //                                                      branchKeyVersion,
-  //                                                      timestamp,
-  //                                                      logicalKeyStoreName,
-  //                                                      KMSKeystoreOperations.GetKeyId(kmsConfiguration),
-  //                                                      customEncryptionContext
-  //                                                    );
-
-  //             //= aws-encryption-sdk-specification/framework/branch-key-store.md#logical-keystore-name
-  //             //= type=implication
-  //             //# The logical keystore name MUST be bound to every created key.
-  //             && decryptOnlyEncryptionContext[Structure.TABLE_FIELD] == logicalKeyStoreName
-
-  //             // TODO-HV-2-M1: Refactor EncryptionContext usage into BranchKeyContext
-  //             //= aws-encryption-sdk-specification/framework/branch-key-store.md#encryption-context
-  //             //= type=implication
-  //             //# Any additionally attributes in the EncryptionContext
-  //             //# of the [encrypted hierarchical key](./key-store/key-storage.md#encryptedhierarchicalkey)
-  //             //# MUST be added to the encryption context.
-  //             && (forall k <- customEncryptionContext
-  //                   ::
-  //                     && Structure.ENCRYPTION_CONTEXT_PREFIX + k in decryptOnlyEncryptionContext
-  //                     && decryptOnlyEncryptionContext[Structure.ENCRYPTION_CONTEXT_PREFIX + k] == customEncryptionContext[k])
-
-  //   // //= aws-encryption-sdk-specification/framework/branch-key-store.md#branch-key-and-beacon-key-creation
-  //   // //= type=implication
-  //   // //# The wrapped Branch Keys, DECRYPT_ONLY and ACTIVE, MUST be created according to [Wrapped Branch Key Creation](#wrapped-branch-key-creation).
-  //   // && WrappedBranchKeyCreation?(
-  //   //      Seq.Last(kmsClient.History.Encrypt),
-  //   //      kmsClient,
-  //   //      kmsConfiguration,
-  //   //      grantTokens,
-  //   //      decryptOnlyEncryptionContext
-  //   //    )
-
-
-  //   // //= aws-encryption-sdk-specification/framework/branch-key-store.md#branch-key-and-beacon-key-creation
-  //   // //= type=implication
-  //   // //# The operation MUST call [AWS KMS API GenerateDataKeyWithoutPlaintext](https://docs.aws.amazon.com/kms/latest/APIReference/API_GenerateDataKeyWithoutPlaintext.html).
-  //   // && var beaconKmsRequest := Seq.Last(kmsClient.History.GenerateDataKeyWithoutPlaintext);
-
-  //   //           //= aws-encryption-sdk-specification/framework/branch-key-store.md#branch-key-and-beacon-key-creation
-  //   //           //= type=implication
-  //   //           //# The operation MUST call AWS KMS GenerateDataKeyWithoutPlaintext with a request constructed as follows:
-  //   //           && var beaconKmsInput := beaconKmsRequest.input;
-
-  //   //           //= aws-encryption-sdk-specification/framework/branch-key-store.md#branch-key-and-beacon-key-creation
-  //   //           //= type=implication
-  //   //           //# - `KeyId` MUST be [compatible with](#aws-key-arn-compatibility) the configured KMS Key in the [AWS KMS Configuration](#aws-kms-configuration) for this keystore.
-  //   //           && KMSKeystoreOperations.Compatible?(kmsConfiguration, beaconKmsInput.KeyId)
-
-  //   //           //= aws-encryption-sdk-specification/framework/branch-key-store.md#branch-key-and-beacon-key-creation
-  //   //           //= type=implication
-  //   //           //# - `NumberOfBytes` MUST be 32.
-  //   //           && beaconKmsInput.NumberOfBytes == Some(32)
-
-  //   //           //= aws-encryption-sdk-specification/framework/branch-key-store.md#branch-key-and-beacon-key-creation
-  //   //           //= type=implication
-  //   //           //# - `EncryptionContext` MUST be the [encryption context for beacon keys](#beacon-key-encryption-context).
-  //   //           && beaconKmsInput.EncryptionContext == Some(Structure.BeaconKeyEncryptionContext(decryptOnlyEncryptionContext))
-
-  //   //           //= aws-encryption-sdk-specification/framework/branch-key-store.md#branch-key-and-beacon-key-creation
-  //   //           //= type=implication
-  //   //           //# - `GrantTokens` MUST be this keystore's [grant tokens](https://docs.aws.amazon.com/kms/latest/developerguide/concepts.html#grant_token).
-  //   //           && beaconKmsInput.GrantTokens == Some(grantTokens)
-
-  //   //           && beaconKmsRequest.output.Success?
-  //   //           && beaconKmsRequest.output.value.CiphertextBlob.Some?
-
-  //   //           && |storage.History.WriteNewEncryptedBranchKey| == |old(storage.History.WriteNewEncryptedBranchKey)| + 1
-
-  //   //           && Seq.Last(storage.History.WriteNewEncryptedBranchKey).input.Active
-  //   //              == Structure.ConstructEncryptedHierarchicalKey(
-  //   //                   Seq.Last(kmsClient.History.ReEncrypt).input.DestinationEncryptionContext.value,
-  //   //                   //= aws-encryption-sdk-specification/framework/branch-key-store.md#wrapped-branch-key-creation
-  //   //                   //= type=implication
-  //   //                   //# If the call to AWS KMS ReEncrypt succeeds,
-  //   //                   //# the operation MUST use the ReEncrypt result `CiphertextBlob`
-  //   //                   //# as the wrapped ACTIVE Branch Key.
-  //   //                   Seq.Last(kmsClient.History.ReEncrypt).output.value.CiphertextBlob.value
-  //   //                 )
-
-  //   //           && Seq.Last(storage.History.WriteNewEncryptedBranchKey).input.Version
-  //   //              == Structure.ConstructEncryptedHierarchicalKey(
-  //   //                   Seq.Last(Seq.DropLast(kmsClient.History.GenerateDataKeyWithoutPlaintext)).input.EncryptionContext.value,
-  //   //                   //= aws-encryption-sdk-specification/framework/branch-key-store.md#wrapped-branch-key-creation
-  //   //                   //= type=implication
-  //   //                   //# If the call to AWS KMS GenerateDataKeyWithoutPlaintext succeeds,
-  //   //                   //# the operation MUST use the GenerateDataKeyWithoutPlaintext result `CiphertextBlob`
-  //   //                   //# as the wrapped DECRYPT_ONLY Branch Key.
-  //   //                   Seq.Last(Seq.DropLast(kmsClient.History.GenerateDataKeyWithoutPlaintext)).output.value.CiphertextBlob.value
-  //   //                 )
-
-  //   //           && Seq.Last(storage.History.WriteNewEncryptedBranchKey).input.Beacon
-  //   //              == Structure.ConstructEncryptedHierarchicalKey(
-  //   //                   Seq.Last(kmsClient.History.GenerateDataKeyWithoutPlaintext).input.EncryptionContext.value,
-  //   //                   //= aws-encryption-sdk-specification/framework/branch-key-store.md#branch-key-and-beacon-key-creation
-  //   //                   //= type=implication
-  //   //                   //# If the call to AWS KMS GenerateDataKeyWithoutPlaintext succeeds,
-  //   //                   //# the operation MUST use the `CiphertextBlob` as the wrapped Beacon Key.
-  //   //                   Seq.Last(kmsClient.History.GenerateDataKeyWithoutPlaintext).output.value.CiphertextBlob.value
-  //   //                 )
-
-  //   //           && Seq.Last(storage.History.WriteNewEncryptedBranchKey).output.Success?
-
-  //   // //= aws-encryption-sdk-specification/framework/branch-key-store.md#createkey
-  //   // //= type=implication
-  //   // //# If creation of the keys are successful,
-  //   // //# then the key store MUST call the configured [KeyStorage interface's](./key-store/key-storage.md#interface)
-  //   // //# [WriteNewEncryptedBranchKey](./key-store/key-storage.md#writenewencryptedbranchkey) with these 3 [EncryptedHierarchicalKeys](./key-store/key-storage.md#encryptedhierarchicalkey).
-  //   // ensures
-  //   //   && output.Success?
-  //   //   && |kmsClient.History.GenerateDataKeyWithoutPlaintext| == |old(kmsClient.History.GenerateDataKeyWithoutPlaintext)| + 2
-  //   //   && |kmsClient.History.ReEncrypt| == |old(kmsClient.History.ReEncrypt)| + 1
-  //   //   && Seq.Last(Seq.DropLast(kmsClient.History.GenerateDataKeyWithoutPlaintext)).output.Success?
-  //   //   && Seq.Last(kmsClient.History.GenerateDataKeyWithoutPlaintext).output.Success?
-  //   //   && Seq.Last(kmsClient.History.ReEncrypt).output.Success?
-  //   //   ==>
-  //   //     && |storage.History.WriteNewEncryptedBranchKey| == |old(storage.History.WriteNewEncryptedBranchKey)| + 1
-
-  //   // //= aws-encryption-sdk-specification/framework/branch-key-store.md#createkey
-  //   // //= type=implication
-  //   // //# If writing to the keystore succeeds,
-  //   // //# the operation MUST return the branch-key-id that maps to both
-  //   // //# the branch key and the beacon key.
-  //   // ensures
-  //   //   && |storage.History.WriteNewEncryptedBranchKey| == |old(storage.History.WriteNewEncryptedBranchKey)| + 1
-  //   //   && Seq.Last(storage.History.WriteNewEncryptedBranchKey).output.Success?
-  //   //   ==>
-  //   //     && output.Success?
-  //   //     && output.value.branchKeyIdentifier == branchKeyIdentifier
-
-
-  //   // //= aws-encryption-sdk-specification/framework/branch-key-store.md#createkey
-  //   // //= type=implication
-  //   // //# Otherwise, this operation MUST yield an error.
-  //   // ensures
-
-  //   //   || (&& |kmsClient.History.GenerateDataKeyWithoutPlaintext| == |old(kmsClient.History.GenerateDataKeyWithoutPlaintext)| + 1
-  //   //       && Seq.Last(kmsClient.History.GenerateDataKeyWithoutPlaintext).output.Failure?
-  //   //       ==> output.Failure?)
-
-  //   //   || (&& |kmsClient.History.ReEncrypt| == |old(kmsClient.History.ReEncrypt)| + 1
-  //   //       && Seq.Last(kmsClient.History.ReEncrypt).output.Failure?
-  //   //       ==> output.Failure?)
-
-  //   //   || (&& |kmsClient.History.GenerateDataKeyWithoutPlaintext| == |old(kmsClient.History.GenerateDataKeyWithoutPlaintext)| + 2
-  //   //       && Seq.Last(kmsClient.History.GenerateDataKeyWithoutPlaintext).output.Failure?
-  //   //       ==> output.Failure?)
-
-  //   //   || (&& |storage.History.WriteNewEncryptedBranchKey| == |old(storage.History.WriteNewEncryptedBranchKey)| + 1
-  //   //       && Seq.Last(storage.History.WriteNewEncryptedBranchKey).output.Failure?
-  //   //       ==> output.Failure?)
-
-  // {
-
-  //   var decryptOnlyEncryptionContext := Structure.DecryptOnlyBranchKeyEncryptionContext(
-  //     branchKeyIdentifier,
-  //     branchKeyVersion,
-  //     timestamp,
-  //     logicalKeyStoreName,
-  //     KMSKeystoreOperations.GetKeyId(kmsConfiguration),
-  //     customEncryptionContext
-  //   );
-  //   var activeEncryptionContext := Structure.ActiveBranchKeyEncryptionContext(decryptOnlyEncryptionContext);
-  //   var beaconEncryptionContext := Structure.BeaconKeyEncryptionContext(decryptOnlyEncryptionContext);
-
-  //   assert KMSKeystoreOperations.AttemptKmsOperation?(kmsConfiguration, decryptOnlyEncryptionContext[Structure.KMS_FIELD]);
-  //   var wrappedDecryptOnlyBranchKey :- KMSKeystoreOperations.GenerateKey(
-  //     decryptOnlyEncryptionContext,
-  //     kmsConfiguration,
-  //     grantTokens,
-  //     kmsClient
-  //   );
-  //   assert KMSKeystoreOperations.AttemptKmsOperation?(kmsConfiguration, activeEncryptionContext[Structure.KMS_FIELD]);
-  //   var wrappedActiveBranchKey :- KMSKeystoreOperations.ReEncryptKey(
-  //     wrappedDecryptOnlyBranchKey.CiphertextBlob.value,
-  //     decryptOnlyEncryptionContext,
-  //     activeEncryptionContext,
-  //     kmsConfiguration,
-  //     grantTokens,
-  //     kmsClient
-  //   );
-  //   assert KMSKeystoreOperations.AttemptKmsOperation?(kmsConfiguration, beaconEncryptionContext[Structure.KMS_FIELD]);
-  //   var wrappedBeaconKey :- KMSKeystoreOperations.GenerateKey(
-  //     beaconEncryptionContext,
-  //     kmsConfiguration,
-  //     grantTokens,
-  //     kmsClient
-  //   );
-
-  //   var _ :- storage.WriteNewEncryptedBranchKey(
-  //     Types.WriteNewEncryptedBranchKeyInput(
-  //       Active := Structure.ConstructEncryptedHierarchicalKey(
-  //         activeEncryptionContext,
-  //         wrappedActiveBranchKey.CiphertextBlob.value
-  //       ),
-  //       Version := Structure.ConstructEncryptedHierarchicalKey(
-  //         decryptOnlyEncryptionContext,
-  //         wrappedDecryptOnlyBranchKey.CiphertextBlob.value
-  //       ),
-  //       Beacon := Structure.ConstructEncryptedHierarchicalKey(
-  //         beaconEncryptionContext,
-  //         wrappedBeaconKey.CiphertextBlob.value
-  //       )
-  //     )
-  //   );
-
-  //   output := Success(
-  //     Types.CreateKeyOutput(
-  //       branchKeyIdentifier := branchKeyIdentifier
-  //     ));
-  // }
-
-  // method VersionActiveBranchKey(
-  //   input: Types.VersionKeyInput,
-  //   timestamp: string,
-  //   branchKeyVersion: string,
-  //   logicalKeyStoreName: string,
-  //   kmsConfiguration: Types.KMSConfiguration,
-  //   grantTokens: KMS.GrantTokenList,
-  //   kmsClient: KMS.IKMSClient,
-  //   storage: Types.IKeyStorageInterface
-  // )
-  //   returns (output: Result<Types.VersionKeyOutput, Types.Error>)
-  //   requires 0 < |input.branchKeyIdentifier| && 0 < |branchKeyVersion|
-  //   requires storage.Modifies !! kmsClient.Modifies
-  //   requires KMSKeystoreOperations.HasKeyId(kmsConfiguration) && KmsArn.ValidKmsArn?(KMSKeystoreOperations.GetKeyId(kmsConfiguration))
-  //   requires storage is DefaultKeyStorageInterface.DynamoDBKeyStorageInterface
-  //            ==>
-  //              logicalKeyStoreName == (storage as DefaultKeyStorageInterface.DynamoDBKeyStorageInterface).logicalKeyStoreName
-
-  //   requires kmsClient.ValidState() && storage.ValidState()
-  //   modifies storage.Modifies, kmsClient.Modifies
-  //   ensures storage.ValidState() && kmsClient.ValidState()
-
-  //   //= aws-encryption-sdk-specification/framework/branch-key-store.md#versionkey
-  //   //= type=implication
-  //   //# VersionKey MUST first get the active version for the branch key from the keystore
-  //   //# by calling the configured [KeyStorage interface's](./key-store/key-storage.md#interface)
-  //   //# [GetEncryptedActiveBranchKey](./key-store/key-storage.md#getencryptedactivebranchkey)
-  //   //# using the `branch-key-id`.
-  //   ensures
-  //     && |storage.History.GetEncryptedActiveBranchKey| == |old(storage.History.GetEncryptedActiveBranchKey)| + 1
-  //     && Seq.Last(storage.History.GetEncryptedActiveBranchKey).input.Identifier == input.branchKeyIdentifier
-
-  //   ensures output.Success?
-  //           ==>
-  //             && Seq.Last(storage.History.GetEncryptedActiveBranchKey).output.Success?
-  //             && var oldActiveItem := Seq.Last(storage.History.GetEncryptedActiveBranchKey).output.value.Item;
-
-
-  //             //= aws-encryption-sdk-specification/framework/branch-key-store.md#versionkey
-  //             //= type=implication
-  //             //# VersionKey MUST verify that the returned EncryptedHierarchicalKey MUST have the requested `branch-key-id`.
-  //             && oldActiveItem.Identifier == input.branchKeyIdentifier
-
-  //             //= aws-encryption-sdk-specification/framework/branch-key-store.md#versionkey
-  //             //= type=implication
-  //             //# VersionKey MUST verify that the returned EncryptedHierarchicalKey is an ActiveHierarchicalSymmetricVersion.
-  //             && Structure.ActiveHierarchicalSymmetricKey?(oldActiveItem)
-
-  //             //= aws-encryption-sdk-specification/framework/branch-key-store.md#versionkey
-  //             //= type=implication
-  //             //# VersionKey MUST verify that the returned EncryptedHierarchicalKey MUST have a logical table name equal to the configured logical table name.
-  //             && oldActiveItem.EncryptionContext[Structure.TABLE_FIELD] == logicalKeyStoreName
-
-  //             //= aws-encryption-sdk-specification/framework/branch-key-store.md#versionkey
-  //             //= type=implication
-  //             //# The `KmsArn` of the [EncryptedHierarchicalKey](./key-store/key-storage.md#encryptedhierarchicalkey)
-  //             //# MUST be [compatible with](#aws-key-arn-compatibility)
-  //             //# the configured `KMS ARN` in the [AWS KMS Configuration](#aws-kms-configuration) for this keystore.
-  //             && KMSKeystoreOperations.AttemptKmsOperation?(kmsConfiguration, oldActiveItem.EncryptionContext[Structure.KMS_FIELD])
-  //             && KMSKeystoreOperations.Compatible?(kmsConfiguration, oldActiveItem.KmsArn)
-
-  //             //= aws-encryption-sdk-specification/framework/branch-key-store.md#versionkey
-  //             //= type=implication
-  //             //# The [EncryptedHierarchicalKey](./key-store/key-storage.md#encryptedhierarchicalkey)
-  //             //# MUST be authenticated according to [authenticating a keystore item](#authenticating-an-encryptedhierarchicalkey).
-
-  //             // TODO-HV-2-M1: Verify CreateKeyOutput?
-  //             // //= aws-encryption-sdk-specification/framework/branch-key-store.md#authenticating-an-encryptedhierarchicalkey
-  //             // //= type=implication
-  //             // //# The operation MUST use the configured `KMS SDK Client` to authenticate the value of the keystore item.
-  //             // && |kmsClient.History.Encrypt| == |old(kmsClient.History.Encrypt)| + 3
-
-  //             // //= aws-encryption-sdk-specification/framework/branch-key-store.md#authenticating-an-encryptedhierarchicalkey
-  //             // //= type=implication
-  //             // //# The operation MUST call [AWS KMS API ReEncrypt](https://docs.aws.amazon.com/kms/latest/APIReference/API_ReEncrypt.html)
-  //             // //# with a request constructed as follows:
-  //             // && var reEncryptInput := Seq.Last(Seq.DropLast(kmsClient.History.ReEncrypt)).input;
-
-  //             // //= aws-encryption-sdk-specification/framework/branch-key-store.md#authenticating-an-encryptedhierarchicalkey
-  //             // //= type=implication
-  //             // //# - `SourceEncryptionContext` MUST be the [encryption context](#encryption-context) of the EncryptedHierarchicalKey to be authenticated
-  //             // && reEncryptInput.SourceEncryptionContext == Some(oldActiveItem.EncryptionContext)
-
-  //             // //= aws-encryption-sdk-specification/framework/branch-key-store.md#authenticating-an-encryptedhierarchicalkey
-  //             // //= type=implication
-  //             // //# - `SourceKeyId` MUST be [compatible with](#aws-key-arn-compatibility) the configured KMS Key in the [AWS KMS Configuration](#aws-kms-configuration) for this keystore.
-  //             // && KMSKeystoreOperations.OptCompatible?(kmsConfiguration, reEncryptInput.SourceKeyId)
-
-  //             // //= aws-encryption-sdk-specification/framework/branch-key-store.md#authenticating-an-encryptedhierarchicalkey
-  //             // //= type=implication
-  //             // //# - `CiphertextBlob` MUST be the `CiphertextBlob` attribute value on the EncryptedHierarchicalKey to be authenticated
-  //             // && reEncryptInput.CiphertextBlob == oldActiveItem.CiphertextBlob
-
-  //             // //= aws-encryption-sdk-specification/framework/branch-key-store.md#authenticating-an-encryptedhierarchicalkey
-  //             // //= type=implication
-  //             // //# - `GrantTokens` MUST be the configured [grant tokens](https://docs.aws.amazon.com/kms/latest/developerguide/concepts.html#grant_token).
-  //             // && reEncryptInput.GrantTokens == Some(grantTokens)
-
-  //             // //= aws-encryption-sdk-specification/framework/branch-key-store.md#authenticating-an-encryptedhierarchicalkey
-  //             // //= type=implication
-  //             // //# - `DestinationKeyId` MUST be [compatible with](#aws-key-arn-compatibility) the configured KMS Key in the [AWS KMS Configuration](#aws-kms-configuration) for this keystore.
-  //             // && KMSKeystoreOperations.Compatible?(kmsConfiguration, reEncryptInput.DestinationKeyId)
-
-  //             // //= aws-encryption-sdk-specification/framework/branch-key-store.md#authenticating-an-encryptedhierarchicalkey
-  //             // //= type=implication
-  //             // //# - `DestinationEncryptionContext` MUST be the [encryption context](#encryption-context) of the EncryptedHierarchicalKey to be authenticated
-  //             // && reEncryptInput.DestinationEncryptionContext == Some(oldActiveItem.EncryptionContext)
-
-  //             // && |kmsClient.History.GenerateDataKeyWithoutPlaintext| == |old(kmsClient.History.GenerateDataKeyWithoutPlaintext)| + 1
-  //             // && old(kmsClient.History.GenerateDataKeyWithoutPlaintext) < kmsClient.History.GenerateDataKeyWithoutPlaintext
-  //             // && old(kmsClient.History.ReEncrypt) < kmsClient.History.ReEncrypt
-
-  //             // && var decryptOnlyEncryptionContext := Structure.NewVersionFromActiveBranchKeyEncryptionContext(
-  //             //                                          oldActiveItem.EncryptionContext,
-  //             //                                          branchKeyVersion,
-  //             //                                          timestamp
-  //             //                                        );
-
-  //             // TODO-HV-2-M1-FF: Add Predicate?
-  //             // //= aws-encryption-sdk-specification/framework/branch-key-store.md#versionkey
-  //             // //= type=implication
-  //             // //# The wrapped Branch Keys, DECRYPT_ONLY and ACTIVE, MUST be created according to [Wrapped Branch Key Creation](#wrapped-branch-key-creation).
-  //             // && WrappedBranchKeyCreation?(
-  //             //      Seq.Last(kmsClient.History.GenerateDataKeyWithoutPlaintext),
-  //             //      Seq.Last(kmsClient.History.ReEncrypt),
-  //             //      kmsClient,
-  //             //      kmsConfiguration,
-  //             //      grantTokens,
-  //             //      decryptOnlyEncryptionContext
-  //             //    )
-
-  //             && |storage.History.WriteNewEncryptedBranchKeyVersion| == |old(storage.History.WriteNewEncryptedBranchKeyVersion)| + 1
-
-  //             // TODO-HV-2-M1: Verify Storage Calls
-  //             // //= aws-encryption-sdk-specification/framework/branch-key-store.md#versionkey
-  //             // //= type=implication
-  //             // //# If creation of the keys are successful,
-  //             // //# then the key store MUST call the configured [KeyStorage interface's](./key-store/key-storage.md#interface)
-  //             // //# [WriteNewEncryptedBranchKeyVersion](./key-store/key-storage.md##writenewencryptedbranchkeyversion)
-  //             // //# with these 2 [EncryptedHierarchicalKeys](./key-store/key-storage.md##encryptedhierarchicalkey).
-  //             // && Seq.Last(storage.History.WriteNewEncryptedBranchKeyVersion).input.Active.Item
-  //             //    == Structure.ConstructEncryptedHierarchicalKey(
-  //             //         Seq.Last(kmsClient.History.ReEncrypt).input.DestinationEncryptionContext.value,
-  //             //         Seq.Last(kmsClient.History.ReEncrypt).output.value.CiphertextBlob.value
-  //             //       )
-
-  //             // && Seq.Last(storage.History.WriteNewEncryptedBranchKeyVersion).input.Version
-  //             //    == Structure.ConstructEncryptedHierarchicalKey(
-  //             //         Seq.Last(kmsClient.History.GenerateDataKeyWithoutPlaintext).input.EncryptionContext.value,
-  //             //         Seq.Last(kmsClient.History.GenerateDataKeyWithoutPlaintext).output.value.CiphertextBlob.value
-  //             //       )
-
-  //             //= aws-encryption-sdk-specification/framework/branch-key-store.md#versionkey
-  //             //= type=implication
-  //             //# The `kms-arn` stored in the table MUST NOT change as a result of this operation,
-  //             //# even if the KeyStore is configured with a `KMS MRKey ARN` that does not exactly match the stored ARN.
-  //             && Seq.Last(storage.History.WriteNewEncryptedBranchKeyVersion).input.Active.Item.KmsArn == oldActiveItem.KmsArn
-  //             && Seq.Last(storage.History.WriteNewEncryptedBranchKeyVersion).input.Version.KmsArn == oldActiveItem.KmsArn
-
-  //             && Seq.Last(storage.History.WriteNewEncryptedBranchKeyVersion).output.Success?
-
-
-  //             //= aws-encryption-sdk-specification/framework/branch-key-store.md#versionkey
-  //             //= type=implication
-  //             //# If the [WriteNewEncryptedBranchKeyVersion](./key-store/key-storage.md#writenewencryptedbranchkeyversion) is successful,
-  //             //# this operation MUST return a successful response containing no additional data.
-  //             && output == Success(Types.VersionKeyOutput)
-
-  //   // TODO-HV-2-M1: Ensure Verification according to Encrypt/Decrypt Strategy
-  //   ensures
-  //     //= aws-encryption-sdk-specification/framework/branch-key-store.md#versionkey
-  //     //= type=implication
-  //     //# If the item fails to authenticate this operation MUST fail.
-  //     || (&& |kmsClient.History.Encrypt| == |old(kmsClient.History.Encrypt)| + 1
-  //         && Seq.Last(kmsClient.History.Encrypt).output.Failure?
-  //         ==> output.Failure?)
-
-  //     || (&& |kmsClient.History.Encrypt| == |old(kmsClient.History.Encrypt)| + 2
-  //         && Seq.Last(Seq.DropLast(kmsClient.History.Encrypt)).output.Failure?
-  //         ==> output.Failure?)
-
-  //     || (&& |kmsClient.History.Encrypt| == |old(kmsClient.History.Encrypt)| + 3
-  //         && Seq.Last(Seq.DropLast(Seq.DropLast(kmsClient.History.Encrypt))).output.Failure?
-  //         ==> output.Failure?)
-
-  //     || (&& |storage.History.GetEncryptedActiveBranchKey| == |old(storage.History.GetEncryptedActiveBranchKey)| + 1
-  //         && Seq.Last(storage.History.WriteNewEncryptedBranchKeyVersion).output.Failure?
-  //         ==> output.Failure?)
-
-  //     || (&& |storage.History.WriteNewEncryptedBranchKeyVersion| == |old(storage.History.WriteNewEncryptedBranchKeyVersion)| + 1
-  //         && Seq.Last(storage.History.WriteNewEncryptedBranchKeyVersion).output.Failure?
-  //         ==> output.Failure?)
-
-  // {
-
-  //   var GetEncryptedActiveBranchKeyOutput :- storage.GetEncryptedActiveBranchKey(
-  //     Types.GetEncryptedActiveBranchKeyInput(
-  //       Identifier := input.branchKeyIdentifier
-  //     )
-  //   );
-  //   var oldActiveItem := GetEncryptedActiveBranchKeyOutput.Item;
-
-  //   :- Need(
-  //     || storage is DefaultKeyStorageInterface.DynamoDBKeyStorageInterface
-  //     || (
-  //          && oldActiveItem.Identifier == input.branchKeyIdentifier
-  //          && Structure.ActiveHierarchicalSymmetricKey?(oldActiveItem)
-  //          && oldActiveItem.EncryptionContext[Structure.TABLE_FIELD] == logicalKeyStoreName
-  //        ),
-  //     Types.KeyStoreException(
-  //       message := ErrorMessages.INVALID_ACTIVE_BRANCH_KEY_FROM_STORAGE)
-  //   );
-  //   // TODO-HV-2-M3: Support Version in HV-2
-  //   :- Need(
-  //     oldActiveItem.EncryptionContext[Structure.HIERARCHY_VERSION] == Structure.HIERARCHY_VERSION_VALUE_1,
-  //     Types.KeyStoreException(
-  //       message := "At this time, VersionKey ONLY supports HV-1; BK's Active Item is HV-2.")
-  //   );
-  //   :- Need(
-  //     && KMSKeystoreOperations.AttemptKmsOperation?(kmsConfiguration, oldActiveItem.EncryptionContext[Structure.KMS_FIELD]),
-  //     Types.KeyStoreException(
-  //       message := ErrorMessages.VERSION_KEY_KMS_KEY_ARN_DISAGREEMENT)
-  //   );
-
-  //   var _ :- KMSKeystoreOperations.ReEncryptKey(
-  //     oldActiveItem.CiphertextBlob,
-  //     oldActiveItem.EncryptionContext,
-  //     oldActiveItem.EncryptionContext,
-  //     kmsConfiguration,
-  //     grantTokens,
-  //     kmsClient
-  //   );
-
-  //   var decryptOnlyEncryptionContext := Structure.NewVersionFromActiveBranchKeyEncryptionContext(
-  //     oldActiveItem.EncryptionContext,
-  //     branchKeyVersion,
-  //     timestamp
-  //   );
-
-  //   var activeEncryptionContext := Structure.ActiveBranchKeyEncryptionContext(decryptOnlyEncryptionContext);
-
-  //   assert KMSKeystoreOperations.AttemptKmsOperation?(kmsConfiguration, decryptOnlyEncryptionContext[Structure.KMS_FIELD]);
-
-  //   var wrappedDecryptOnlyBranchKey :- KMSKeystoreOperations.GenerateKey(
-  //     decryptOnlyEncryptionContext,
-  //     kmsConfiguration,
-  //     grantTokens,
-  //     kmsClient
-  //   );
-  //   var wrappedActiveBranchKey :- KMSKeystoreOperations.ReEncryptKey(
-  //     wrappedDecryptOnlyBranchKey.CiphertextBlob.value,
-  //     decryptOnlyEncryptionContext,
-  //     activeEncryptionContext,
-  //     kmsConfiguration,
-  //     grantTokens,
-  //     kmsClient
-  //   );
-
-  //   var active := Structure.ConstructEncryptedHierarchicalKey(
-  //     activeEncryptionContext,
-  //     wrappedActiveBranchKey.CiphertextBlob.value
-  //   );
-  //   var overWrite := Types.OverWriteEncryptedHierarchicalKey(
-  //     Item := active,
-  //     Old := oldActiveItem
-  //   );
-
-  //   var _ :- storage.WriteNewEncryptedBranchKeyVersion(
-  //     Types.WriteNewEncryptedBranchKeyVersionInput(
-  //       Active := overWrite,
-  //       Version :=  Structure.ConstructEncryptedHierarchicalKey(
-  //         decryptOnlyEncryptionContext,
-  //         wrappedDecryptOnlyBranchKey.CiphertextBlob.value
-  //       )
-  //     )
-  //   );
-
-  //   output := Success(Types.VersionKeyOutput());
-  // }
-
-
-  // twostate predicate WrappedBranchKeyCreation?(
-  //   new decryptOnlyEncryptHistory: KMS.DafnyCallEvent<KMS.EncryptRequest, Result<KMS.EncryptResponse, KMS.Error>>,
-  //   new activeEncryptHistory: KMS.DafnyCallEvent<KMS.EncryptRequest, Result<KMS.EncryptResponse, KMS.Error>>,
-  //   kmsClient: KMS.IKMSClient,
-  //   kmsConfiguration: Types.KMSConfiguration,
-  //   grantTokens: KMS.GrantTokenList,
-  //   decryptOnlyEncryptionContext: map<string, string>
-  // )
-  //   reads kmsClient.History
-  //   requires KMSKeystoreOperations.HasKeyId(kmsConfiguration) && KmsArn.ValidKmsArn?(KMSKeystoreOperations.GetKeyId(kmsConfiguration))
-
-
-  //   // The history elements are "the things I added"
-  //   requires old(kmsClient.History.GenerateDataKeyWithoutPlaintext) < kmsClient.History.GenerateDataKeyWithoutPlaintext
-  //   requires old(kmsClient.History.Encrypt) < kmsClient.History.Encrypt
-
-  //   //= aws-encryption-sdk-specification/framework/branch-key-store.md#wrapped-branch-key-creation
-  //   //= type=implication
-  //   //# The call to AWS KMS Encrypt MUST use the configured AWS KMS client to make the call.
-  //   requires
-  //     && encryptHistory in kmsClient.History.Encrypt[|old(kmsClient.History.Encrypt)|..]
-  // {
-
-  //   //= aws-encryption-sdk-specification/framework/branch-key-store.md#wrapped-branch-key-creation
-  //   //= type=implication
-  //   //# The operation MUST call AWS KMS GenerateDataKeyWithoutPlaintext with a request constructed as follows:
-  //   && var decryptOnlyKmsInput := generateHistory.input;
-
-  //   //= aws-encryption-sdk-specification/framework/branch-key-store.md#wrapped-branch-key-creation
-  //   //= type=implication
-  //   //# - `KeyId` MUST be [compatible with](#aws-key-arn-compatibility) the configured KMS Key in the [AWS KMS Configuration](#aws-kms-configuration) for this keystore.
-  //   && KMSKeystoreOperations.Compatible?(kmsConfiguration, decryptOnlyKmsInput.KeyId)
-
-  //   //= aws-encryption-sdk-specification/framework/branch-key-store.md#wrapped-branch-key-creation
-  //   //= type=implication
-  //   //# - `NumberOfBytes` MUST be 32.
-  //   && decryptOnlyKmsInput.NumberOfBytes == Some(32)
-
-  //   //= aws-encryption-sdk-specification/framework/branch-key-store.md#wrapped-branch-key-creation
-  //   //= type=implication
-  //   //# - `EncryptionContext` MUST be the [DECRYPT_ONLY encryption context for branch keys](#decrypt_only-encryption-context).
-  //   && Structure.BranchKeyContext?(decryptOnlyEncryptionContext)
-  //   && decryptOnlyKmsInput.EncryptionContext == Some(decryptOnlyEncryptionContext)
-
-  //   //= aws-encryption-sdk-specification/framework/branch-key-store.md#wrapped-branch-key-creation
-  //   //= type=implication
-  //   //# - GenerateDataKeyWithoutPlaintext `GrantTokens` MUST be this keystore's [grant tokens](https://docs.aws.amazon.com/kms/latest/developerguide/concepts.html#grant_token).
-  //   && decryptOnlyKmsInput.GrantTokens == Some(grantTokens)
-
-  //   && generateHistory.output.Success?
-  //   && generateHistory.output.value.CiphertextBlob.Some?
-
-  //   //= aws-encryption-sdk-specification/framework/branch-key-store.md#wrapped-branch-key-creation
-  //   //= type=implication
-  //   //# The operation MUST call [AWS KMS API ReEncrypt](https://docs.aws.amazon.com/kms/latest/APIReference/API_ReEncrypt.html)
-  //   //# with a request constructed as follows:
-  //   && var activeInput := reEncryptHistory.input;
-
-  //   //= aws-encryption-sdk-specification/framework/branch-key-store.md#wrapped-branch-key-creation
-  //   //= type=implication
-  //   //# - `SourceKeyId` MUST be [compatible with](#aws-key-arn-compatibility) the configured KMS Key in the [AWS KMS Configuration](#aws-kms-configuration) for this keystore.
-  //   && KMSKeystoreOperations.OptCompatible?(kmsConfiguration, activeInput.SourceKeyId)
-
-  //   //= aws-encryption-sdk-specification/framework/branch-key-store.md#wrapped-branch-key-creation
-  //   //= type=implication
-  //   //# - `DestinationKeyId` MUST be [compatible with](#aws-key-arn-compatibility) the configured KMS Key in the [AWS KMS Configuration](#aws-kms-configuration) for this keystore.
-  //   && KMSKeystoreOperations.Compatible?(kmsConfiguration, activeInput.DestinationKeyId)
-
-  //   //= aws-encryption-sdk-specification/framework/branch-key-store.md#wrapped-branch-key-creation
-  //   //= type=implication
-  //   //# - ReEncrypt `GrantTokens` MUST be this keystore's [grant tokens](https://docs.aws.amazon.com/kms/latest/developerguide/concepts.html#grant_token).
-  //   && activeInput.GrantTokens == Some(grantTokens)
-
-  //   //= aws-encryption-sdk-specification/framework/branch-key-store.md#wrapped-branch-key-creation
-  //   //= type=implication
-  //   //# - `CiphertextBlob` MUST be the wrapped DECRYPT_ONLY Branch Key.
-  //   && activeInput.CiphertextBlob == generateHistory.output.value.CiphertextBlob.value
-
-  //   //= aws-encryption-sdk-specification/framework/branch-key-store.md#wrapped-branch-key-creation
-  //   //= type=implication
-  //   //# - `SourceEncryptionContext` MUST be the [DECRYPT_ONLY encryption context for branch keys](#decrypt_only-encryption-context).
-  //   && activeInput.SourceEncryptionContext == Some(decryptOnlyEncryptionContext)
-
-  //   && Structure.BRANCH_KEY_TYPE_PREFIX < decryptOnlyEncryptionContext[Structure.TYPE_FIELD]
-  //   && Structure.BRANCH_KEY_ACTIVE_VERSION_FIELD !in decryptOnlyEncryptionContext
-
-  //   //= aws-encryption-sdk-specification/framework/branch-key-store.md#wrapped-branch-key-creation
-  //   //= type=implication
-  //   //# - `DestinationEncryptionContext` MUST be the [ACTIVE encryption context for branch keys](#active-encryption-context).
-  //   && activeInput.DestinationEncryptionContext == Some(Structure.ActiveBranchKeyEncryptionContext(decryptOnlyEncryptionContext))
-
-  //   && reEncryptHistory.output.Success?
-  //   && reEncryptHistory.output.value.CiphertextBlob.Some?
-
-  // }
+  //= aws-encryption-sdk-specification/framework/branch-key-store.md#branch-key-and-beacon-key-creation
+  //= type=implication
+  //# To create a branch key, this operation MUST take the following:
+  //#
+  //# - `branchKeyId`: The identifier
+  //# - `encryptionContext`: Additional encryption context to bind to the created keys
+  method CreateBranchAndBeaconKeys(
+    branchKeyIdentifier: string,
+    customEncryptionContext: map<string, string>,
+    timestamp: string,
+    branchKeyVersion: string,
+    logicalKeyStoreName: string,
+    kmsConfiguration: Types.KMSConfiguration,
+    grantTokens: KMS.GrantTokenList,
+    kmsClient: KMS.IKMSClient,
+    storage: Types.IKeyStorageInterface
+  )
+    returns (output: Result<Types.CreateKeyOutput, Types.Error>)
+    requires 0 < |branchKeyIdentifier|
+    requires 0 < |branchKeyVersion|
+    requires forall k <- customEncryptionContext :: DDB.IsValid_AttributeName(Structure.ENCRYPTION_CONTEXT_PREFIX + k)
+    requires storage.Modifies !! kmsClient.Modifies
+    requires KMSKeystoreOperations.HasKeyId(kmsConfiguration) && KmsArn.ValidKmsArn?(KMSKeystoreOperations.GetKeyId(kmsConfiguration))
+
+    requires kmsClient.ValidState() && storage.ValidState()
+    modifies storage.Modifies, kmsClient.Modifies
+    ensures storage.ValidState() && kmsClient.ValidState()
+
+    // TODO-HV-2-M1: Update Create Key
+    //= aws-encryption-sdk-specification/framework/branch-key-store.md#createkey
+    //= type=implication
+    //# This operation MUST create a [branch key](structures.md#branch-key) and a [beacon key](structures.md#beacon-key) according to
+    //# the [Branch Key and Beacon Key Creation](#branch-key-and-beacon-key-creation) section.
+    ensures output.Success?
+            ==>
+
+              //= aws-encryption-sdk-specification/framework/branch-key-store.md#branch-key-and-beacon-key-creation
+              //= type=implication
+              //# The call to AWS KMS GenerateDataKeyWithoutPlaintext MUST use the configured AWS KMS client to make the call.
+              // The second call is for the beacon key, the first call is the decrypt only. See Seq.Last(Seq.DropLast(
+              && |kmsClient.History.Encrypt| == |old(kmsClient.History.Encrypt)| + 3
+              && old(kmsClient.History.Encrypt) < kmsClient.History.Encrypt
+
+              // TODO-HV-2-M1-FF: Refactor EncryptionContext usage into BranchKeyContext
+              && var decryptOnlyEncryptionContext := Structure.DecryptOnlyBranchKeyEncryptionContext(
+                                                       branchKeyIdentifier,
+                                                       branchKeyVersion,
+                                                       timestamp,
+                                                       logicalKeyStoreName,
+                                                       KMSKeystoreOperations.GetKeyId(kmsConfiguration),
+                                                       customEncryptionContext
+                                                     );
+
+              //= aws-encryption-sdk-specification/framework/branch-key-store.md#logical-keystore-name
+              //= type=implication
+              //# The logical keystore name MUST be bound to every created key.
+              && decryptOnlyEncryptionContext[Structure.TABLE_FIELD] == logicalKeyStoreName
+
+              // TODO-HV-2-M1: Refactor EncryptionContext usage into BranchKeyContext
+              //= aws-encryption-sdk-specification/framework/branch-key-store.md#encryption-context
+              //= type=implication
+              //# Any additionally attributes in the EncryptionContext
+              //# of the [encrypted hierarchical key](./key-store/key-storage.md#encryptedhierarchicalkey)
+              //# MUST be added to the encryption context.
+              && (forall k <- customEncryptionContext
+                    ::
+                      && Structure.ENCRYPTION_CONTEXT_PREFIX + k in decryptOnlyEncryptionContext
+                      && decryptOnlyEncryptionContext[Structure.ENCRYPTION_CONTEXT_PREFIX + k] == customEncryptionContext[k])
+
+    // //= aws-encryption-sdk-specification/framework/branch-key-store.md#branch-key-and-beacon-key-creation
+    // //= type=implication
+    // //# The wrapped Branch Keys, DECRYPT_ONLY and ACTIVE, MUST be created according to [Wrapped Branch Key Creation](#wrapped-branch-key-creation).
+    // && WrappedBranchKeyCreation?(
+    //      Seq.Last(kmsClient.History.Encrypt),
+    //      kmsClient,
+    //      kmsConfiguration,
+    //      grantTokens,
+    //      decryptOnlyEncryptionContext
+    //    )
+
+
+    // //= aws-encryption-sdk-specification/framework/branch-key-store.md#branch-key-and-beacon-key-creation
+    // //= type=implication
+    // //# The operation MUST call [AWS KMS API GenerateDataKeyWithoutPlaintext](https://docs.aws.amazon.com/kms/latest/APIReference/API_GenerateDataKeyWithoutPlaintext.html).
+    // && var beaconKmsRequest := Seq.Last(kmsClient.History.GenerateDataKeyWithoutPlaintext);
+
+    //           //= aws-encryption-sdk-specification/framework/branch-key-store.md#branch-key-and-beacon-key-creation
+    //           //= type=implication
+    //           //# The operation MUST call AWS KMS GenerateDataKeyWithoutPlaintext with a request constructed as follows:
+    //           && var beaconKmsInput := beaconKmsRequest.input;
+
+    //           //= aws-encryption-sdk-specification/framework/branch-key-store.md#branch-key-and-beacon-key-creation
+    //           //= type=implication
+    //           //# - `KeyId` MUST be [compatible with](#aws-key-arn-compatibility) the configured KMS Key in the [AWS KMS Configuration](#aws-kms-configuration) for this keystore.
+    //           && KMSKeystoreOperations.Compatible?(kmsConfiguration, beaconKmsInput.KeyId)
+
+    //           //= aws-encryption-sdk-specification/framework/branch-key-store.md#branch-key-and-beacon-key-creation
+    //           //= type=implication
+    //           //# - `NumberOfBytes` MUST be 32.
+    //           && beaconKmsInput.NumberOfBytes == Some(32)
+
+    //           //= aws-encryption-sdk-specification/framework/branch-key-store.md#branch-key-and-beacon-key-creation
+    //           //= type=implication
+    //           //# - `EncryptionContext` MUST be the [encryption context for beacon keys](#beacon-key-encryption-context).
+    //           && beaconKmsInput.EncryptionContext == Some(Structure.BeaconKeyEncryptionContext(decryptOnlyEncryptionContext))
+
+    //           //= aws-encryption-sdk-specification/framework/branch-key-store.md#branch-key-and-beacon-key-creation
+    //           //= type=implication
+    //           //# - `GrantTokens` MUST be this keystore's [grant tokens](https://docs.aws.amazon.com/kms/latest/developerguide/concepts.html#grant_token).
+    //           && beaconKmsInput.GrantTokens == Some(grantTokens)
+
+    //           && beaconKmsRequest.output.Success?
+    //           && beaconKmsRequest.output.value.CiphertextBlob.Some?
+
+    //           && |storage.History.WriteNewEncryptedBranchKey| == |old(storage.History.WriteNewEncryptedBranchKey)| + 1
+
+    //           && Seq.Last(storage.History.WriteNewEncryptedBranchKey).input.Active
+    //              == Structure.ConstructEncryptedHierarchicalKey(
+    //                   Seq.Last(kmsClient.History.ReEncrypt).input.DestinationEncryptionContext.value,
+    //                   //= aws-encryption-sdk-specification/framework/branch-key-store.md#wrapped-branch-key-creation
+    //                   //= type=implication
+    //                   //# If the call to AWS KMS ReEncrypt succeeds,
+    //                   //# the operation MUST use the ReEncrypt result `CiphertextBlob`
+    //                   //# as the wrapped ACTIVE Branch Key.
+    //                   Seq.Last(kmsClient.History.ReEncrypt).output.value.CiphertextBlob.value
+    //                 )
+
+    //           && Seq.Last(storage.History.WriteNewEncryptedBranchKey).input.Version
+    //              == Structure.ConstructEncryptedHierarchicalKey(
+    //                   Seq.Last(Seq.DropLast(kmsClient.History.GenerateDataKeyWithoutPlaintext)).input.EncryptionContext.value,
+    //                   //= aws-encryption-sdk-specification/framework/branch-key-store.md#wrapped-branch-key-creation
+    //                   //= type=implication
+    //                   //# If the call to AWS KMS GenerateDataKeyWithoutPlaintext succeeds,
+    //                   //# the operation MUST use the GenerateDataKeyWithoutPlaintext result `CiphertextBlob`
+    //                   //# as the wrapped DECRYPT_ONLY Branch Key.
+    //                   Seq.Last(Seq.DropLast(kmsClient.History.GenerateDataKeyWithoutPlaintext)).output.value.CiphertextBlob.value
+    //                 )
+
+    //           && Seq.Last(storage.History.WriteNewEncryptedBranchKey).input.Beacon
+    //              == Structure.ConstructEncryptedHierarchicalKey(
+    //                   Seq.Last(kmsClient.History.GenerateDataKeyWithoutPlaintext).input.EncryptionContext.value,
+    //                   //= aws-encryption-sdk-specification/framework/branch-key-store.md#branch-key-and-beacon-key-creation
+    //                   //= type=implication
+    //                   //# If the call to AWS KMS GenerateDataKeyWithoutPlaintext succeeds,
+    //                   //# the operation MUST use the `CiphertextBlob` as the wrapped Beacon Key.
+    //                   Seq.Last(kmsClient.History.GenerateDataKeyWithoutPlaintext).output.value.CiphertextBlob.value
+    //                 )
+
+    //           && Seq.Last(storage.History.WriteNewEncryptedBranchKey).output.Success?
+
+    // //= aws-encryption-sdk-specification/framework/branch-key-store.md#createkey
+    // //= type=implication
+    // //# If creation of the keys are successful,
+    // //# then the key store MUST call the configured [KeyStorage interface's](./key-store/key-storage.md#interface)
+    // //# [WriteNewEncryptedBranchKey](./key-store/key-storage.md#writenewencryptedbranchkey) with these 3 [EncryptedHierarchicalKeys](./key-store/key-storage.md#encryptedhierarchicalkey).
+    // ensures
+    //   && output.Success?
+    //   && |kmsClient.History.GenerateDataKeyWithoutPlaintext| == |old(kmsClient.History.GenerateDataKeyWithoutPlaintext)| + 2
+    //   && |kmsClient.History.ReEncrypt| == |old(kmsClient.History.ReEncrypt)| + 1
+    //   && Seq.Last(Seq.DropLast(kmsClient.History.GenerateDataKeyWithoutPlaintext)).output.Success?
+    //   && Seq.Last(kmsClient.History.GenerateDataKeyWithoutPlaintext).output.Success?
+    //   && Seq.Last(kmsClient.History.ReEncrypt).output.Success?
+    //   ==>
+    //     && |storage.History.WriteNewEncryptedBranchKey| == |old(storage.History.WriteNewEncryptedBranchKey)| + 1
+
+    // //= aws-encryption-sdk-specification/framework/branch-key-store.md#createkey
+    // //= type=implication
+    // //# If writing to the keystore succeeds,
+    // //# the operation MUST return the branch-key-id that maps to both
+    // //# the branch key and the beacon key.
+    // ensures
+    //   && |storage.History.WriteNewEncryptedBranchKey| == |old(storage.History.WriteNewEncryptedBranchKey)| + 1
+    //   && Seq.Last(storage.History.WriteNewEncryptedBranchKey).output.Success?
+    //   ==>
+    //     && output.Success?
+    //     && output.value.branchKeyIdentifier == branchKeyIdentifier
+
+
+    // //= aws-encryption-sdk-specification/framework/branch-key-store.md#createkey
+    // //= type=implication
+    // //# Otherwise, this operation MUST yield an error.
+    // ensures
+
+    //   || (&& |kmsClient.History.GenerateDataKeyWithoutPlaintext| == |old(kmsClient.History.GenerateDataKeyWithoutPlaintext)| + 1
+    //       && Seq.Last(kmsClient.History.GenerateDataKeyWithoutPlaintext).output.Failure?
+    //       ==> output.Failure?)
+
+    //   || (&& |kmsClient.History.ReEncrypt| == |old(kmsClient.History.ReEncrypt)| + 1
+    //       && Seq.Last(kmsClient.History.ReEncrypt).output.Failure?
+    //       ==> output.Failure?)
+
+    //   || (&& |kmsClient.History.GenerateDataKeyWithoutPlaintext| == |old(kmsClient.History.GenerateDataKeyWithoutPlaintext)| + 2
+    //       && Seq.Last(kmsClient.History.GenerateDataKeyWithoutPlaintext).output.Failure?
+    //       ==> output.Failure?)
+
+    //   || (&& |storage.History.WriteNewEncryptedBranchKey| == |old(storage.History.WriteNewEncryptedBranchKey)| + 1
+    //       && Seq.Last(storage.History.WriteNewEncryptedBranchKey).output.Failure?
+    //       ==> output.Failure?)
+
+  {
+
+    var decryptOnlyEncryptionContext := Structure.DecryptOnlyBranchKeyEncryptionContext(
+      branchKeyIdentifier,
+      branchKeyVersion,
+      timestamp,
+      logicalKeyStoreName,
+      KMSKeystoreOperations.GetKeyId(kmsConfiguration),
+      customEncryptionContext
+    );
+    var activeEncryptionContext := Structure.ActiveBranchKeyEncryptionContext(decryptOnlyEncryptionContext);
+    var beaconEncryptionContext := Structure.BeaconKeyEncryptionContext(decryptOnlyEncryptionContext);
+
+    assert KMSKeystoreOperations.AttemptKmsOperation?(kmsConfiguration, decryptOnlyEncryptionContext[Structure.KMS_FIELD]);
+    var wrappedDecryptOnlyBranchKey :- KMSKeystoreOperations.GenerateKey(
+      decryptOnlyEncryptionContext,
+      kmsConfiguration,
+      grantTokens,
+      kmsClient
+    );
+    assert KMSKeystoreOperations.AttemptKmsOperation?(kmsConfiguration, activeEncryptionContext[Structure.KMS_FIELD]);
+    var wrappedActiveBranchKey :- KMSKeystoreOperations.ReEncryptKey(
+      wrappedDecryptOnlyBranchKey.CiphertextBlob.value,
+      decryptOnlyEncryptionContext,
+      activeEncryptionContext,
+      kmsConfiguration,
+      grantTokens,
+      kmsClient
+    );
+    assert KMSKeystoreOperations.AttemptKmsOperation?(kmsConfiguration, beaconEncryptionContext[Structure.KMS_FIELD]);
+    var wrappedBeaconKey :- KMSKeystoreOperations.GenerateKey(
+      beaconEncryptionContext,
+      kmsConfiguration,
+      grantTokens,
+      kmsClient
+    );
+
+    var _ :- storage.WriteNewEncryptedBranchKey(
+      Types.WriteNewEncryptedBranchKeyInput(
+        Active := Structure.ConstructEncryptedHierarchicalKey(
+          activeEncryptionContext,
+          wrappedActiveBranchKey.CiphertextBlob.value
+        ),
+        Version := Structure.ConstructEncryptedHierarchicalKey(
+          decryptOnlyEncryptionContext,
+          wrappedDecryptOnlyBranchKey.CiphertextBlob.value
+        ),
+        Beacon := Structure.ConstructEncryptedHierarchicalKey(
+          beaconEncryptionContext,
+          wrappedBeaconKey.CiphertextBlob.value
+        )
+      )
+    );
+
+    output := Success(
+      Types.CreateKeyOutput(
+        branchKeyIdentifier := branchKeyIdentifier
+      ));
+  }
+
+  method VersionActiveBranchKey(
+    input: Types.VersionKeyInput,
+    timestamp: string,
+    branchKeyVersion: string,
+    logicalKeyStoreName: string,
+    kmsConfiguration: Types.KMSConfiguration,
+    grantTokens: KMS.GrantTokenList,
+    kmsClient: KMS.IKMSClient,
+    storage: Types.IKeyStorageInterface
+  )
+    returns (output: Result<Types.VersionKeyOutput, Types.Error>)
+    requires 0 < |input.branchKeyIdentifier| && 0 < |branchKeyVersion|
+    requires storage.Modifies !! kmsClient.Modifies
+    requires KMSKeystoreOperations.HasKeyId(kmsConfiguration) && KmsArn.ValidKmsArn?(KMSKeystoreOperations.GetKeyId(kmsConfiguration))
+    requires storage is DefaultKeyStorageInterface.DynamoDBKeyStorageInterface
+             ==>
+               logicalKeyStoreName == (storage as DefaultKeyStorageInterface.DynamoDBKeyStorageInterface).logicalKeyStoreName
+
+    requires kmsClient.ValidState() && storage.ValidState()
+    modifies storage.Modifies, kmsClient.Modifies
+    ensures storage.ValidState() && kmsClient.ValidState()
+
+    //= aws-encryption-sdk-specification/framework/branch-key-store.md#versionkey
+    //= type=implication
+    //# VersionKey MUST first get the active version for the branch key from the keystore
+    //# by calling the configured [KeyStorage interface's](./key-store/key-storage.md#interface)
+    //# [GetEncryptedActiveBranchKey](./key-store/key-storage.md#getencryptedactivebranchkey)
+    //# using the `branch-key-id`.
+    ensures
+      && |storage.History.GetEncryptedActiveBranchKey| == |old(storage.History.GetEncryptedActiveBranchKey)| + 1
+      && Seq.Last(storage.History.GetEncryptedActiveBranchKey).input.Identifier == input.branchKeyIdentifier
+
+    ensures output.Success?
+            ==>
+              && Seq.Last(storage.History.GetEncryptedActiveBranchKey).output.Success?
+              && var oldActiveItem := Seq.Last(storage.History.GetEncryptedActiveBranchKey).output.value.Item;
+
+
+              //= aws-encryption-sdk-specification/framework/branch-key-store.md#versionkey
+              //= type=implication
+              //# VersionKey MUST verify that the returned EncryptedHierarchicalKey MUST have the requested `branch-key-id`.
+              && oldActiveItem.Identifier == input.branchKeyIdentifier
+
+              //= aws-encryption-sdk-specification/framework/branch-key-store.md#versionkey
+              //= type=implication
+              //# VersionKey MUST verify that the returned EncryptedHierarchicalKey is an ActiveHierarchicalSymmetricVersion.
+              && Structure.ActiveHierarchicalSymmetricKey?(oldActiveItem)
+
+              //= aws-encryption-sdk-specification/framework/branch-key-store.md#versionkey
+              //= type=implication
+              //# VersionKey MUST verify that the returned EncryptedHierarchicalKey MUST have a logical table name equal to the configured logical table name.
+              && oldActiveItem.EncryptionContext[Structure.TABLE_FIELD] == logicalKeyStoreName
+
+              //= aws-encryption-sdk-specification/framework/branch-key-store.md#versionkey
+              //= type=implication
+              //# The `KmsArn` of the [EncryptedHierarchicalKey](./key-store/key-storage.md#encryptedhierarchicalkey)
+              //# MUST be [compatible with](#aws-key-arn-compatibility)
+              //# the configured `KMS ARN` in the [AWS KMS Configuration](#aws-kms-configuration) for this keystore.
+              && KMSKeystoreOperations.AttemptKmsOperation?(kmsConfiguration, oldActiveItem.EncryptionContext[Structure.KMS_FIELD])
+              && KMSKeystoreOperations.Compatible?(kmsConfiguration, oldActiveItem.KmsArn)
+
+              //= aws-encryption-sdk-specification/framework/branch-key-store.md#versionkey
+              //= type=implication
+              //# The [EncryptedHierarchicalKey](./key-store/key-storage.md#encryptedhierarchicalkey)
+              //# MUST be authenticated according to [authenticating a keystore item](#authenticating-an-encryptedhierarchicalkey).
+
+              // TODO-HV-2-M1: Verify CreateKeyOutput?
+              // //= aws-encryption-sdk-specification/framework/branch-key-store.md#authenticating-an-encryptedhierarchicalkey
+              // //= type=implication
+              // //# The operation MUST use the configured `KMS SDK Client` to authenticate the value of the keystore item.
+              // && |kmsClient.History.Encrypt| == |old(kmsClient.History.Encrypt)| + 3
+
+              // //= aws-encryption-sdk-specification/framework/branch-key-store.md#authenticating-an-encryptedhierarchicalkey
+              // //= type=implication
+              // //# The operation MUST call [AWS KMS API ReEncrypt](https://docs.aws.amazon.com/kms/latest/APIReference/API_ReEncrypt.html)
+              // //# with a request constructed as follows:
+              // && var reEncryptInput := Seq.Last(Seq.DropLast(kmsClient.History.ReEncrypt)).input;
+
+              // //= aws-encryption-sdk-specification/framework/branch-key-store.md#authenticating-an-encryptedhierarchicalkey
+              // //= type=implication
+              // //# - `SourceEncryptionContext` MUST be the [encryption context](#encryption-context) of the EncryptedHierarchicalKey to be authenticated
+              // && reEncryptInput.SourceEncryptionContext == Some(oldActiveItem.EncryptionContext)
+
+              // //= aws-encryption-sdk-specification/framework/branch-key-store.md#authenticating-an-encryptedhierarchicalkey
+              // //= type=implication
+              // //# - `SourceKeyId` MUST be [compatible with](#aws-key-arn-compatibility) the configured KMS Key in the [AWS KMS Configuration](#aws-kms-configuration) for this keystore.
+              // && KMSKeystoreOperations.OptCompatible?(kmsConfiguration, reEncryptInput.SourceKeyId)
+
+              // //= aws-encryption-sdk-specification/framework/branch-key-store.md#authenticating-an-encryptedhierarchicalkey
+              // //= type=implication
+              // //# - `CiphertextBlob` MUST be the `CiphertextBlob` attribute value on the EncryptedHierarchicalKey to be authenticated
+              // && reEncryptInput.CiphertextBlob == oldActiveItem.CiphertextBlob
+
+              // //= aws-encryption-sdk-specification/framework/branch-key-store.md#authenticating-an-encryptedhierarchicalkey
+              // //= type=implication
+              // //# - `GrantTokens` MUST be the configured [grant tokens](https://docs.aws.amazon.com/kms/latest/developerguide/concepts.html#grant_token).
+              // && reEncryptInput.GrantTokens == Some(grantTokens)
+
+              // //= aws-encryption-sdk-specification/framework/branch-key-store.md#authenticating-an-encryptedhierarchicalkey
+              // //= type=implication
+              // //# - `DestinationKeyId` MUST be [compatible with](#aws-key-arn-compatibility) the configured KMS Key in the [AWS KMS Configuration](#aws-kms-configuration) for this keystore.
+              // && KMSKeystoreOperations.Compatible?(kmsConfiguration, reEncryptInput.DestinationKeyId)
+
+              // //= aws-encryption-sdk-specification/framework/branch-key-store.md#authenticating-an-encryptedhierarchicalkey
+              // //= type=implication
+              // //# - `DestinationEncryptionContext` MUST be the [encryption context](#encryption-context) of the EncryptedHierarchicalKey to be authenticated
+              // && reEncryptInput.DestinationEncryptionContext == Some(oldActiveItem.EncryptionContext)
+
+              // && |kmsClient.History.GenerateDataKeyWithoutPlaintext| == |old(kmsClient.History.GenerateDataKeyWithoutPlaintext)| + 1
+              // && old(kmsClient.History.GenerateDataKeyWithoutPlaintext) < kmsClient.History.GenerateDataKeyWithoutPlaintext
+              // && old(kmsClient.History.ReEncrypt) < kmsClient.History.ReEncrypt
+
+              // && var decryptOnlyEncryptionContext := Structure.NewVersionFromActiveBranchKeyEncryptionContext(
+              //                                          oldActiveItem.EncryptionContext,
+              //                                          branchKeyVersion,
+              //                                          timestamp
+              //                                        );
+
+              // TODO-HV-2-M1-FF: Add Predicate?
+              // //= aws-encryption-sdk-specification/framework/branch-key-store.md#versionkey
+              // //= type=implication
+              // //# The wrapped Branch Keys, DECRYPT_ONLY and ACTIVE, MUST be created according to [Wrapped Branch Key Creation](#wrapped-branch-key-creation).
+              // && WrappedBranchKeyCreation?(
+              //      Seq.Last(kmsClient.History.GenerateDataKeyWithoutPlaintext),
+              //      Seq.Last(kmsClient.History.ReEncrypt),
+              //      kmsClient,
+              //      kmsConfiguration,
+              //      grantTokens,
+              //      decryptOnlyEncryptionContext
+              //    )
+
+              && |storage.History.WriteNewEncryptedBranchKeyVersion| == |old(storage.History.WriteNewEncryptedBranchKeyVersion)| + 1
+
+              // TODO-HV-2-M1: Verify Storage Calls
+              // //= aws-encryption-sdk-specification/framework/branch-key-store.md#versionkey
+              // //= type=implication
+              // //# If creation of the keys are successful,
+              // //# then the key store MUST call the configured [KeyStorage interface's](./key-store/key-storage.md#interface)
+              // //# [WriteNewEncryptedBranchKeyVersion](./key-store/key-storage.md##writenewencryptedbranchkeyversion)
+              // //# with these 2 [EncryptedHierarchicalKeys](./key-store/key-storage.md##encryptedhierarchicalkey).
+              // && Seq.Last(storage.History.WriteNewEncryptedBranchKeyVersion).input.Active.Item
+              //    == Structure.ConstructEncryptedHierarchicalKey(
+              //         Seq.Last(kmsClient.History.ReEncrypt).input.DestinationEncryptionContext.value,
+              //         Seq.Last(kmsClient.History.ReEncrypt).output.value.CiphertextBlob.value
+              //       )
+
+              // && Seq.Last(storage.History.WriteNewEncryptedBranchKeyVersion).input.Version
+              //    == Structure.ConstructEncryptedHierarchicalKey(
+              //         Seq.Last(kmsClient.History.GenerateDataKeyWithoutPlaintext).input.EncryptionContext.value,
+              //         Seq.Last(kmsClient.History.GenerateDataKeyWithoutPlaintext).output.value.CiphertextBlob.value
+              //       )
+
+              //= aws-encryption-sdk-specification/framework/branch-key-store.md#versionkey
+              //= type=implication
+              //# The `kms-arn` stored in the table MUST NOT change as a result of this operation,
+              //# even if the KeyStore is configured with a `KMS MRKey ARN` that does not exactly match the stored ARN.
+              && Seq.Last(storage.History.WriteNewEncryptedBranchKeyVersion).input.Active.Item.KmsArn == oldActiveItem.KmsArn
+              && Seq.Last(storage.History.WriteNewEncryptedBranchKeyVersion).input.Version.KmsArn == oldActiveItem.KmsArn
+
+              && Seq.Last(storage.History.WriteNewEncryptedBranchKeyVersion).output.Success?
+
+
+              //= aws-encryption-sdk-specification/framework/branch-key-store.md#versionkey
+              //= type=implication
+              //# If the [WriteNewEncryptedBranchKeyVersion](./key-store/key-storage.md#writenewencryptedbranchkeyversion) is successful,
+              //# this operation MUST return a successful response containing no additional data.
+              && output == Success(Types.VersionKeyOutput)
+
+    // TODO-HV-2-M1: Ensure Verification according to Encrypt/Decrypt Strategy
+    ensures
+      //= aws-encryption-sdk-specification/framework/branch-key-store.md#versionkey
+      //= type=implication
+      //# If the item fails to authenticate this operation MUST fail.
+      || (&& |kmsClient.History.Encrypt| == |old(kmsClient.History.Encrypt)| + 1
+          && Seq.Last(kmsClient.History.Encrypt).output.Failure?
+          ==> output.Failure?)
+
+      || (&& |kmsClient.History.Encrypt| == |old(kmsClient.History.Encrypt)| + 2
+          && Seq.Last(Seq.DropLast(kmsClient.History.Encrypt)).output.Failure?
+          ==> output.Failure?)
+
+      || (&& |kmsClient.History.Encrypt| == |old(kmsClient.History.Encrypt)| + 3
+          && Seq.Last(Seq.DropLast(Seq.DropLast(kmsClient.History.Encrypt))).output.Failure?
+          ==> output.Failure?)
+
+      || (&& |storage.History.GetEncryptedActiveBranchKey| == |old(storage.History.GetEncryptedActiveBranchKey)| + 1
+          && Seq.Last(storage.History.WriteNewEncryptedBranchKeyVersion).output.Failure?
+          ==> output.Failure?)
+
+      || (&& |storage.History.WriteNewEncryptedBranchKeyVersion| == |old(storage.History.WriteNewEncryptedBranchKeyVersion)| + 1
+          && Seq.Last(storage.History.WriteNewEncryptedBranchKeyVersion).output.Failure?
+          ==> output.Failure?)
+
+  {
+
+    var GetEncryptedActiveBranchKeyOutput :- storage.GetEncryptedActiveBranchKey(
+      Types.GetEncryptedActiveBranchKeyInput(
+        Identifier := input.branchKeyIdentifier
+      )
+    );
+    var oldActiveItem := GetEncryptedActiveBranchKeyOutput.Item;
+
+    :- Need(
+      || storage is DefaultKeyStorageInterface.DynamoDBKeyStorageInterface
+      || (
+           && oldActiveItem.Identifier == input.branchKeyIdentifier
+           && Structure.ActiveHierarchicalSymmetricKey?(oldActiveItem)
+           && oldActiveItem.EncryptionContext[Structure.TABLE_FIELD] == logicalKeyStoreName
+         ),
+      Types.KeyStoreException(
+        message := ErrorMessages.INVALID_ACTIVE_BRANCH_KEY_FROM_STORAGE)
+    );
+    // TODO-HV-2-M3: Support Version in HV-2
+    :- Need(
+      oldActiveItem.EncryptionContext[Structure.HIERARCHY_VERSION] == Structure.HIERARCHY_VERSION_VALUE_1,
+      Types.KeyStoreException(
+        message := "At this time, VersionKey ONLY supports HV-1; BK's Active Item is HV-2.")
+    );
+    :- Need(
+      && KMSKeystoreOperations.AttemptKmsOperation?(kmsConfiguration, oldActiveItem.EncryptionContext[Structure.KMS_FIELD]),
+      Types.KeyStoreException(
+        message := ErrorMessages.VERSION_KEY_KMS_KEY_ARN_DISAGREEMENT)
+    );
+
+    var _ :- KMSKeystoreOperations.ReEncryptKey(
+      oldActiveItem.CiphertextBlob,
+      oldActiveItem.EncryptionContext,
+      oldActiveItem.EncryptionContext,
+      kmsConfiguration,
+      grantTokens,
+      kmsClient
+    );
+
+    var decryptOnlyEncryptionContext := Structure.NewVersionFromActiveBranchKeyEncryptionContext(
+      oldActiveItem.EncryptionContext,
+      branchKeyVersion,
+      timestamp
+    );
+
+    var activeEncryptionContext := Structure.ActiveBranchKeyEncryptionContext(decryptOnlyEncryptionContext);
+
+    assert KMSKeystoreOperations.AttemptKmsOperation?(kmsConfiguration, decryptOnlyEncryptionContext[Structure.KMS_FIELD]);
+
+    var wrappedDecryptOnlyBranchKey :- KMSKeystoreOperations.GenerateKey(
+      decryptOnlyEncryptionContext,
+      kmsConfiguration,
+      grantTokens,
+      kmsClient
+    );
+    var wrappedActiveBranchKey :- KMSKeystoreOperations.ReEncryptKey(
+      wrappedDecryptOnlyBranchKey.CiphertextBlob.value,
+      decryptOnlyEncryptionContext,
+      activeEncryptionContext,
+      kmsConfiguration,
+      grantTokens,
+      kmsClient
+    );
+
+    var active := Structure.ConstructEncryptedHierarchicalKey(
+      activeEncryptionContext,
+      wrappedActiveBranchKey.CiphertextBlob.value
+    );
+    var overWrite := Types.OverWriteEncryptedHierarchicalKey(
+      Item := active,
+      Old := oldActiveItem
+    );
+
+    var _ :- storage.WriteNewEncryptedBranchKeyVersion(
+      Types.WriteNewEncryptedBranchKeyVersionInput(
+        Active := overWrite,
+        Version :=  Structure.ConstructEncryptedHierarchicalKey(
+          decryptOnlyEncryptionContext,
+          wrappedDecryptOnlyBranchKey.CiphertextBlob.value
+        )
+      )
+    );
+
+    output := Success(Types.VersionKeyOutput());
+  }
+
+
+  twostate predicate WrappedBranchKeyCreation?(
+    new decryptOnlyEncryptHistory: KMS.DafnyCallEvent<KMS.EncryptRequest, Result<KMS.EncryptResponse, KMS.Error>>,
+    new activeEncryptHistory: KMS.DafnyCallEvent<KMS.EncryptRequest, Result<KMS.EncryptResponse, KMS.Error>>,
+    kmsClient: KMS.IKMSClient,
+    kmsConfiguration: Types.KMSConfiguration,
+    grantTokens: KMS.GrantTokenList,
+    decryptOnlyEncryptionContext: map<string, string>
+  )
+    reads kmsClient.History
+    requires KMSKeystoreOperations.HasKeyId(kmsConfiguration) && KmsArn.ValidKmsArn?(KMSKeystoreOperations.GetKeyId(kmsConfiguration))
+
+
+    // The history elements are "the things I added"
+    requires old(kmsClient.History.GenerateDataKeyWithoutPlaintext) < kmsClient.History.GenerateDataKeyWithoutPlaintext
+    requires old(kmsClient.History.Encrypt) < kmsClient.History.Encrypt
+
+    //= aws-encryption-sdk-specification/framework/branch-key-store.md#wrapped-branch-key-creation
+    //= type=implication
+    //# The call to AWS KMS Encrypt MUST use the configured AWS KMS client to make the call.
+    requires
+      && encryptHistory in kmsClient.History.Encrypt[|old(kmsClient.History.Encrypt)|..]
+  {
+
+    //= aws-encryption-sdk-specification/framework/branch-key-store.md#wrapped-branch-key-creation
+    //= type=implication
+    //# The operation MUST call AWS KMS GenerateDataKeyWithoutPlaintext with a request constructed as follows:
+    && var decryptOnlyKmsInput := generateHistory.input;
+
+    //= aws-encryption-sdk-specification/framework/branch-key-store.md#wrapped-branch-key-creation
+    //= type=implication
+    //# - `KeyId` MUST be [compatible with](#aws-key-arn-compatibility) the configured KMS Key in the [AWS KMS Configuration](#aws-kms-configuration) for this keystore.
+    && KMSKeystoreOperations.Compatible?(kmsConfiguration, decryptOnlyKmsInput.KeyId)
+
+    //= aws-encryption-sdk-specification/framework/branch-key-store.md#wrapped-branch-key-creation
+    //= type=implication
+    //# - `NumberOfBytes` MUST be 32.
+    && decryptOnlyKmsInput.NumberOfBytes == Some(32)
+
+    //= aws-encryption-sdk-specification/framework/branch-key-store.md#wrapped-branch-key-creation
+    //= type=implication
+    //# - `EncryptionContext` MUST be the [DECRYPT_ONLY encryption context for branch keys](#decrypt_only-encryption-context).
+    && Structure.BranchKeyContext?(decryptOnlyEncryptionContext)
+    && decryptOnlyKmsInput.EncryptionContext == Some(decryptOnlyEncryptionContext)
+
+    //= aws-encryption-sdk-specification/framework/branch-key-store.md#wrapped-branch-key-creation
+    //= type=implication
+    //# - GenerateDataKeyWithoutPlaintext `GrantTokens` MUST be this keystore's [grant tokens](https://docs.aws.amazon.com/kms/latest/developerguide/concepts.html#grant_token).
+    && decryptOnlyKmsInput.GrantTokens == Some(grantTokens)
+
+    && generateHistory.output.Success?
+    && generateHistory.output.value.CiphertextBlob.Some?
+
+    //= aws-encryption-sdk-specification/framework/branch-key-store.md#wrapped-branch-key-creation
+    //= type=implication
+    //# The operation MUST call [AWS KMS API ReEncrypt](https://docs.aws.amazon.com/kms/latest/APIReference/API_ReEncrypt.html)
+    //# with a request constructed as follows:
+    && var activeInput := reEncryptHistory.input;
+
+    //= aws-encryption-sdk-specification/framework/branch-key-store.md#wrapped-branch-key-creation
+    //= type=implication
+    //# - `SourceKeyId` MUST be [compatible with](#aws-key-arn-compatibility) the configured KMS Key in the [AWS KMS Configuration](#aws-kms-configuration) for this keystore.
+    && KMSKeystoreOperations.OptCompatible?(kmsConfiguration, activeInput.SourceKeyId)
+
+    //= aws-encryption-sdk-specification/framework/branch-key-store.md#wrapped-branch-key-creation
+    //= type=implication
+    //# - `DestinationKeyId` MUST be [compatible with](#aws-key-arn-compatibility) the configured KMS Key in the [AWS KMS Configuration](#aws-kms-configuration) for this keystore.
+    && KMSKeystoreOperations.Compatible?(kmsConfiguration, activeInput.DestinationKeyId)
+
+    //= aws-encryption-sdk-specification/framework/branch-key-store.md#wrapped-branch-key-creation
+    //= type=implication
+    //# - ReEncrypt `GrantTokens` MUST be this keystore's [grant tokens](https://docs.aws.amazon.com/kms/latest/developerguide/concepts.html#grant_token).
+    && activeInput.GrantTokens == Some(grantTokens)
+
+    //= aws-encryption-sdk-specification/framework/branch-key-store.md#wrapped-branch-key-creation
+    //= type=implication
+    //# - `CiphertextBlob` MUST be the wrapped DECRYPT_ONLY Branch Key.
+    && activeInput.CiphertextBlob == generateHistory.output.value.CiphertextBlob.value
+
+    //= aws-encryption-sdk-specification/framework/branch-key-store.md#wrapped-branch-key-creation
+    //= type=implication
+    //# - `SourceEncryptionContext` MUST be the [DECRYPT_ONLY encryption context for branch keys](#decrypt_only-encryption-context).
+    && activeInput.SourceEncryptionContext == Some(decryptOnlyEncryptionContext)
+
+    && Structure.BRANCH_KEY_TYPE_PREFIX < decryptOnlyEncryptionContext[Structure.TYPE_FIELD]
+    && Structure.BRANCH_KEY_ACTIVE_VERSION_FIELD !in decryptOnlyEncryptionContext
+
+    //= aws-encryption-sdk-specification/framework/branch-key-store.md#wrapped-branch-key-creation
+    //= type=implication
+    //# - `DestinationEncryptionContext` MUST be the [ACTIVE encryption context for branch keys](#active-encryption-context).
+    && activeInput.DestinationEncryptionContext == Some(Structure.ActiveBranchKeyEncryptionContext(decryptOnlyEncryptionContext))
+
+    && reEncryptHistory.output.Success?
+    && reEncryptHistory.output.value.CiphertextBlob.Some?
+
+  }
 }
